HlistMachine no longer an instance of AbstractMachine

src/Verse/HlistMachine.v
@@ -1,10 +1,25 @@
 (* begin hide *)
+Require Import Verse.Ast.
 Require Import Verse.TypeSystem.
+Require Import Verse.Language.Types.
 Require Import Verse.Scope.
 Require Import Verse.Utils.hlist.
-Require Import Verse.AbstractMachine.
 Require Import Verse.Abstract.Machine.
+Require Import Verse.Monoid.
+Require Import Verse.Monoid.Semantics.
+
+Require Import PeanoNat.
+
+Require Import EqdepFacts.
+Import EqNotations.
+
 (* end hide *)
+
+
+(** Verse code is written universally quantified over the variable
+universe. For the purpose of verification, we instantiate the generic
+Verse code with a "universal" variable dictated by its scope. We can
+also give a computable State for such variables.  *)
 
 Section Hlist.
 
@@ -21,21 +36,178 @@ Section Hlist.
              (genC : forall v, scoped v sc (CODE v)) :=
     uncurry (genC memV) (all_membership sc).
 
-  Instance HlistMem : State memV tyD.
-  refine {| str         := memory tyd sc;
-            val         := fun m _ v => index v m;
-            storeUpdate := fun _ v f m => update v m (f (index v m));
-            evalUpdate  := _;
-         |}.
-  constructor.
-  apply update_other_index.
-  apply updated_index.
-  Defined.
+  Local Definition type := typeOf ts.
+  Let tyd ty := typeTrans tyD (projT2 ty).
 
-  Definition annotation := AbstractMachine.assertion (H := HlistMem).
-  Definition transformation := AbstractMachine.instruction (H := HlistMem).
-  Definition denotation := mline memV tyD HlistMem.
+  Definition str := Machine.memory tyd sc.
+
+  Definition val (m : str) ty (x : memV ty)
+    := index x m.
+
+  Definition update ty (x : memV ty) f (m : str)
+    := update x m (f (index x m)).
+
+  Definition transformation := str -> str.
+
+  Definition assertion := str*str -> Prop.
+
+  Global Instance assertion_action_op : LActionOp transformation assertion :=
+    fun inst ap => fun oAn => ap (fst oAn, inst (snd oAn)).
+
+  Add Parametric Morphism : lact with signature
+      SetoidClass.equiv (A:=transformation) ==> SetoidClass.equiv (A:=assertion) ==> SetoidClass.equiv (A:=assertion) as lact_morp.
+    unfold lact.
+    unfold assertion_action_op; simpl.
+    intros P Q.
+    intro  PEQ.
+    intros tr1 tr2.
+    intro trEq.
+    intro_destruct.
+    rewrite (trEq (s, P s0)).
+    now rewrite PEQ.
+  Qed.
+
+  Global Program Instance assertion_action : LAction transformation assertion :=
+    {| lact_unit := _  |}.
+
+  Next Obligation.
+    intro_destruct; unfold lact. unfold assertion_action_op. intuition.
+  Qed.
+
+  Next Obligation.
+    intro_destruct. unfold lact. unfold assertion_action_op. intuition.
+  Qed.
+
+  Next Obligation.
+    intro_destruct; unfold lact; unfold assertion_action_op. intuition.
+  Qed.
+
+
+  Next Obligation.
+    intro_destruct; unfold lact; unfold assertion_action_op;
+    unfold binop; unfold transition_binop; unfold Basics.compose; simpl. intuition.
+  Qed.
 
 End Hlist.
 
-Arguments fillMemV [ts sc CODE].
+Arguments val [ts sc tyD] _ [ty].
+Arguments update [ts sc tyD ty].
+
+Require Import Verse.TypeSystem.
+
+Section Evaluation.
+  Context {ts : typeSystem}
+          (tyD : typeDenote ts).
+
+  Definition evalLexp {T} (l : lexpr (Variables.sigParam tyD) T)
+    : tyD _ (projT2 T)
+    := match l in (lexpr _ s) return (tyD (projT1 s) (projT2 s)) with
+       | var x => x
+       | @deref _ _ ty b e v idx =>
+           Vector.nth_order
+             (rew [fun T0 : Type@{abstract_type_system.u0} => T0]
+                  arrayCompatibility tyD b e ty
+               in v)
+             (proj2_sig idx)
+       end.
+
+  Fixpoint eval {T} (e : expr (Variables.sigParam tyD) T)
+    :  tyD _ (projT2 T)
+    := match e with
+       | Ast.cval c => constTrans tyD c
+       | Ast.valueOf lv => evalLexp lv
+       | Ast.binOp o e0 e1 => (opTrans tyD o) (eval e0) (eval e1)
+       | Ast.uniOp o e0    => (opTrans tyD o) (eval e0)
+       end.
+End Evaluation.
+
+Module Internals.
+
+  Section MachineType.
+    Variable ts : typeSystem.
+    Variable sc : Scope.type ts.
+    Variable tyD : typeDenote ts.
+
+    Let v := memV sc.
+
+    Definition expr  T := Ast.expr  v T.
+    Definition lexpr T := Ast.lexpr v T.
+
+    Definition evalE {T} (st : str sc tyD) (e : expr T) :  tyD _ (projT2 T)
+      := eval tyD (Expr.rename (val st) e).
+
+    Definition assign {T} (l : lexpr T) (e : expr T)(st : str sc tyD)
+      : str sc tyD :=
+      match l in Ast.lexpr _ T0 return  tyD _ (projT2 T0) -> str _ _ with
+      | Ast.var reg  => fun v => update reg (fun _ => v) st
+      | Ast.deref a idx => fun v => let arr := val st a in
+                                let arrp := Vector.replace_order
+                                              (rew [fun T0 : Type@{abstract_type_system.u0} => T0]
+                                                   arrayCompatibility tyD _ _ _
+                                                in arr)
+                                              (proj2_sig idx) v
+                                in
+                                update a (fun _ =>
+                                            (rew <- [id] arrayCompatibility tyD _ _ _ in arrp)
+                                         ) st
+      end (evalE st e).
+
+    Definition binopUpdate {T}
+               (l : lexpr (existT _ _ T))
+               (o : operator ts T 2)
+               (e : expr (existT _ _ T))
+      : str sc tyD -> str sc tyD
+      := let rhs := Ast.binOp o (Ast.valueOf l) e in
+         assign l rhs.
+
+    Definition uniopUpdate {T}
+               (l : lexpr (existT _ _ T))
+               (o : operator ts T 1)
+      : str sc tyD -> str sc tyD
+      := let rhs := Ast.uniOp o (Ast.valueOf l) in
+         assign l rhs.
+
+    Program Definition move {T}(l : lexpr T)(r : v T) :=
+      match l in Ast.lexpr _ T0 return v T0 -> _ with
+      | var _ as l1     => fun r0 => assign l1 (Ast.valueOf (Ast.var r0))
+      | deref _ _ as l1 => fun r0 => assign l1 (Ast.valueOf (Ast.var r0))
+      end r.
+
+    Definition denoteInst {T}(inst : Ast.instruction v  T) : transformation sc tyD
+      := match inst with
+         | Ast.assign l e => assign l e
+         | Ast.moveTo l r => move   l r
+         | Ast.binopUpdate l o e => binopUpdate l o e
+         | Ast.uniopUpdate l o   => uniopUpdate l o
+         | Ast.clobber _     => fun x => x
+         end.
+
+    Definition denoteStmt (stmt : Ast.statement v) : transformation sc tyD
+      := denoteInst (projT2 stmt).
+
+  End MachineType.
+
+End Internals.
+
+Section Machine.
+
+  Variable ts : typeSystem.
+  Variable sc : Scope.type ts.
+
+  Variable tyD   : typeDenote ts.
+
+  Definition mline := transformation sc tyD ⋉ assertion sc tyD.
+
+  Definition justInst
+    : transformation sc tyD -> mline
+    := fun i => semiR i (fun _ => True).
+
+  Definition justAssert
+    : assertion sc tyD -> mline
+    := fun a => semiR id a.
+
+End Machine.
+
+Arguments mline [ts].
+Arguments justInst [ts sc tyD] .
+Arguments justAssert [ts sc tyD].
